Add peirceOrImpOr'

Logics/ClassicalAxioms/AxiomDef.lean
@@ -38,6 +38,8 @@ def PierceOrLukasiewiczF := fun (a b : Prop) => (((a → b) → a) → a) ∨ ((
 
 def PeirceOrImpOrF := fun (a b : Prop) => (((a → b) → a) → a) ∨ ((a → b) → (¬ a ∨ b))
 
+def PeirceOrImpOrF' := fun (a b : Prop) => (((a → b) → a) → a) ∨ ((b → a) → (¬ b ∨ a))
+
 def DeMorganOrLukasiewiczF := fun (a b : Prop) => (¬ (¬ a ∧ ¬ b) → a ∨ b) ∨ ((¬ a → ¬ b) → (b → a))
 
 def ImpOrOrLukasiewiczF := fun (a b : Prop) => ((a → b) → (¬ a ∨ b)) ∨ ((¬ a → ¬ b) → (b → a))
@@ -82,3 +84,5 @@ def demorganOrLukForm' : Form := .or (demorganForm (.var 0) (.var 1)) (lukForm (
 def impOrOrLukForm' : Form := .or (impOrForm (.var 0) (.var 1)) (lukForm (.var 1) (.var 0))
 
 def peirceOrImpOrForm : Form := .or (peirceForm (.var 0) (.var 1)) (impOrForm (.var 0) (.var 1))
+
+def peirceOrImpOrForm' : Form := .or (peirceForm (.var 0) (.var 1)) (impOrForm (.var 1) (.var 0))
